model/processor/multiprocessor.v
@@ -1,5 +1,6 @@
 From mathcomp Require Export fintype.
 Require Export prosa.behavior.all.
+Require Import prosa.analysis.facts.behavior.service.
 
 (** * Multiprocessor State *)
 
@@ -25,7 +26,7 @@ Section Schedule.
   Context `{ProcessorState Job processor_state}.
 
   (** Given a desired number of processors [num_cpus], we define a finite type
-      of integers from 0 to [num_cpus - 1]. The purpose of this definition is
+      of integers from [0] to [num_cpus - 1]. The purpose of this definition is
       to obtain a finite type (i.e., set of values) that can be enumerated in a
       terminating computation.
 
@@ -43,33 +44,40 @@ Section Schedule.
 
   (** Based on this notion of multiprocessor state, we say that a given job [j]
       is currently scheduled on a specific processor [cpu], according to the
-      given multiprocessor state [mps], if [j] is scheduled in the
-      processor-local state [(mps cpu)].  *)
-  Let multiproc_scheduled_on (j : Job) (mps : multiprocessor_state) (cpu : processor num_cpus)
+      given multiprocessor state [mps], iff [j] is scheduled in the
+      processor-local state [(mps cpu)]. *)
+  Definition multiproc_scheduled_on
+      (j : Job) (mps : multiprocessor_state) (cpu : processor num_cpus)
     := scheduled_in j (mps cpu).
 
-  (** The service received by a given job [j] in a given multiprocessor state
-      [mps] is given by the sum of the service received across all individual
-      processors of the multiprocessor. *)
-  Let multiproc_service_in (j : Job) (mps : multiprocessor_state)
-    := \sum_(cpu < num_cpus) service_in j (mps cpu).
+  (** Similarly, the service received by a given job [j] in a given
+      multiprocessor state [mps] on a given processor of ID [cpu] is exactly
+      the service given by [j] in the processor-local state [(mps cpu)]. *)
+  Definition multiproc_service_on
+      (j : Job) (mps : multiprocessor_state) (cpu : processor num_cpus)
+    := service_in j (mps cpu).
 
   (** Finally, we connect the above definitions with the generic Prosa
       interface for processor models. *)
   Global Program Instance multiproc_state : ProcessorState Job multiprocessor_state :=
     {
       scheduled_on := multiproc_scheduled_on;
-      service_in := multiproc_service_in
+      service_on := multiproc_service_on
     }.
   Next Obligation.
-    move: j s H0.
-    move=> j s /existsP Hsched.
-    apply/eqP.
-    rewrite sum_nat_eq0.
-    apply/forallP=>/= c.
-    rewrite service_implies_scheduled//.
-    case: (boolP (scheduled_in _ _))=>//= Habs.
-    exfalso; apply: Hsched.
-      by exists c.
+    move: j s r H0.
+    move=> j mps cpu.
+    by apply: service_in_implies_scheduled_in.
   Defined.
+
+  (** From the instance [multiproc_state], we get the function [service_in].
+      The service received by a given job [j] in a given multiprocessor state
+      [mps] is given by the sum of the service received across all individual
+      processors of the multiprocessor. *)
+  Lemma multiproc_service_in_eq : forall (j : Job) (mps : multiprocessor_state),
+    service_in j mps = \sum_(cpu < num_cpus) service_in j (mps cpu).
+  Proof.
+    reflexivity.
+  Qed.
+
 End Schedule.
