analysis/facts/model/ideal_schedule.v
@@ -11,11 +11,11 @@ Require Import prosa.model.processor.ideal.
 (** In this section we establish the classes to which an ideal schedule belongs. *)
 Section ScheduleClass.
 
-  Local Transparent service_in scheduled_in scheduled_on.
+  Local Transparent scheduled_in scheduled_on.
   (** Consider any job type and the ideal processor model. *)
   Context {Job: JobType}.
   Context `{JobArrival Job}.
-  Context `{JobCost Job}.  
+  Context `{JobCost Job}.
 
   (** We note that the ideal processor model is indeed a uni-processor
      model. *)
@@ -23,7 +23,30 @@ Section ScheduleClass.
     uniprocessor_model (processor_state Job).
   Proof.
     move=> j1 j2 sched t /existsP[[]/eqP E1] /existsP[[]/eqP E2].
-    by move: E1 E2=>->[].
+    by move: E1 E2 =>->[].
+  Qed.
+
+  (** By definition, [service_in] is the sum of the service received
+      in total across all cores.  In the ideal uniprocessor model,
+      however, there is only one "core," which is expressed by using
+      [unit] as the type of cores. The type [unit] only has a single
+      member [tt], which serves as a placeholder. Consequently, the
+      definition of [service_in] simplifies to a single term of the
+      sum, the service on the one core, which we note with the
+      following lemma that relates [service_in] to [service_on]. *)
+  Lemma service_in_service_on (j : Job) s :
+    service_in j s = service_on j s tt.
+  Proof.
+    by rewrite /service_in /index_enum Finite.EnumDef.enumDef /= big_seq1.
+  Qed.
+
+  (** Furthermore, since the ideal uniprocessor state is represented
+      by the [option Job] type, [service_in] further simplifies to a
+      simple equality comparison, which we note next. *)
+  Lemma service_in_def (j : Job) (s : processor_state Job) :
+    service_in j s = (s == Some j).
+  Proof.
+    by rewrite service_in_service_on.
   Qed.
 
   (** We observe that the ideal processor model falls into the category
@@ -32,8 +55,8 @@ Section ScheduleClass.
   Lemma ideal_proc_model_ensures_ideal_progress:
     ideal_progress_proc_model (processor_state Job).
   Proof.
-    move=> j s /existsP[[]/eqP->]/=.
-    by rewrite eqxx.
+    move=> j s /existsP[[]/eqP->] /=.
+    by rewrite service_in_def /= eqxx /nat_of_bool.
   Qed.
 
   (** The ideal processor model is a unit-service model. *)
@@ -41,7 +64,7 @@ Section ScheduleClass.
     unit_service_proc_model (processor_state Job).
   Proof.
     move=> j s.
-    rewrite /service_in/=/nat_of_bool.
+    rewrite service_in_def /= /nat_of_bool.
     by case:ifP.
   Qed.
 
@@ -51,7 +74,7 @@ Section ScheduleClass.
     rewrite /scheduled_in/scheduled_on/=.
     case: existsP=>[[_->]//|].
     case: (s == Some j)=>//=[[]].
-      by exists.
+    by exists.
   Qed.
 
   Lemma scheduled_at_def sched (j : Job) t :
@@ -63,7 +86,7 @@ Section ScheduleClass.
   Lemma service_in_is_scheduled_in (j : Job) s :
     service_in j s = scheduled_in j s.
   Proof.
-    by rewrite /service_in scheduled_in_def/=.
+    by rewrite service_in_def scheduled_in_def.
   Qed.
 
   Lemma service_at_is_scheduled_at sched (j : Job) t :
@@ -71,19 +94,31 @@ Section ScheduleClass.
   Proof.
       by rewrite /service_at service_in_is_scheduled_in.
   Qed.
-    
+
+  Lemma service_on_def (j : Job) (s : processor_state Job) c :
+    service_on j s c = (s == Some j).
+  Proof.
+    done.
+  Qed.
+
+  Lemma service_at_def sched (j : Job) t :
+    service_at sched j t = (sched t == Some j).
+  Proof.
+    by rewrite /service_at service_in_def.
+  Qed.
+
   (** Next we prove a lemma which helps us to do a case analysis on
    the state of an ideal schedule. *)
   Lemma ideal_proc_model_sched_case_analysis:
     forall (sched : schedule (ideal.processor_state Job)) (t : instant),
-      is_idle sched t \/ exists j, scheduled_at sched j t. 
+      is_idle sched t \/ exists j, scheduled_at sched j t.
   Proof.
     intros.
     unfold is_idle; simpl; destruct (sched t) eqn:EQ.
     - by right; exists s; auto; rewrite scheduled_at_def EQ.
     - by left; auto.
   Qed.
-  
+
 End ScheduleClass.
 
 (** * Incremental Service in Ideal Schedule *)
@@ -100,15 +135,15 @@ Section IncrementalService.
   Variable arr_seq : arrival_sequence Job.
 
   (** ... and any ideal uni-processor schedule of this arrival sequence. *)
-  Variable sched : schedule (ideal.processor_state Job).  
+  Variable sched : schedule (ideal.processor_state Job).
 
-  (** As a base case, we prove that if a job j receives service in
-      some time interval <<[t1,t2)>>, then there exists a time instant t
-      ∈ [t1,t2) such that j is scheduled at time t and t is the first
-      instant where j receives service. *)
+  (** As a base case, we prove that if a job [j] receives service in
+      some time interval <<[t1,t2)>>, then there exists a time instant
+      <<t ∈ [t1,t2)>> such that [j] is scheduled at time [t] and [t] is
+      the first instant where [j] receives service. *)
   Lemma positive_service_during:
     forall j t1 t2,
-      0 < service_during sched j t1 t2 -> 
+      0 < service_during sched j t1 t2 ->
       exists t : nat, t1 <= t < t2 /\ scheduled_at sched j t /\ service_during sched j t1 t = 0.
   Proof.
     intros j t1 t2 SERV.
@@ -121,11 +156,12 @@ Section IncrementalService.
       - apply/andP; split; first by done.
         rewrite ltnNge; apply/negP; intros CONTR.
           by move: SERV; rewrite/service_during big_geq.
-      - by rewrite /service_during big_geq.                
-    }  
+      - by rewrite /service_during big_geq.
+    }
     { apply negbT in SCHED.
-      move: SERV; rewrite /service /service_during; move => /sum_seq_gt0P [t [IN SCHEDt]].
-      rewrite lt0b in SCHEDt.
+      move: SERV.
+      rewrite /service_during => /sum_seq_gt0P [t [IN SCHEDt]].
+      rewrite service_at_def /= lt0b in SCHEDt.
       rewrite mem_iota subnKC in IN; last by done.
       move: IN => /andP [IN1 IN2].
       move: (exists_first_intermediate_point
@@ -134,67 +170,84 @@ Section IncrementalService.
       move: A => [x [/andP [T1 T4] [T2 T3]]].
       exists x; repeat split; try done.
       - apply/andP; split; first by apply ltnW.
-          by apply leq_ltn_trans with t. 
+          by apply leq_ltn_trans with t.
       - apply/eqP; rewrite big_nat_cond big1 //.
         move => y /andP [T5 _].
-          by apply/eqP; rewrite eqb0; specialize (T2 y); rewrite scheduled_at_def/= in T2; apply T2.
+        apply/eqP.
+        rewrite service_at_def /= eqb0.
+        by specialize (T2 y); rewrite scheduled_at_def/= in T2; apply T2.
     }
   Qed.
 
-  (** Next, we prove that if in some time interval <<[t1,t2)>> a job j
-     receives k units of service, then there exists a time instant t ∈
-     [t1,t2) such that j is scheduled at time t and service of job j
-     within interval [t1,t) is equal to k. *)
+  (** Furthermore, we observe that, if a job receives some positive
+      amount of service during an interval <<[t1, t2)>>, then the
+      interval can't be empty and hence [t1 < t2]. *)
+  Lemma service_during_ge :
+    forall j t1 t2 k,
+      service_during sched j t1 t2 > k ->
+      t1 < t2.
+  Proof.
+    move=> j t1 t2 k SERV.
+    rewrite leqNgt.
+    apply/negP => CONTR.
+    move: SERV.
+    by rewrite /service_during big_geq.
+  Qed.
+
+  (** Next, we prove that if in some time interval <<[t1,t2)>> a job [j]
+     receives [k] units of service, then there exists a time instant
+     <<t ∈ [t1,t2)>> such that [j] is scheduled at time [t] and service
+     of job [j] within interval <<[t1,t)>> is equal to [k]. *)
   Lemma incremental_service_during:
     forall j t1 t2 k,
       service_during sched j t1 t2 > k ->
       exists t, t1 <= t < t2 /\ scheduled_at sched j t /\ service_during sched j t1 t = k.
   Proof.
-    intros j t1 t2 k SERV.
-    have LE: t1 <= t2.
-    { rewrite leqNgt; apply/negP; intros CONTR.
-        by apply ltnW in CONTR;  move: SERV; rewrite /service_during big_geq.
-    }
+    move=> j t1 t2 k SERV.
+    have LE: t1 < t2 by move: (service_during_ge _ _ _ _ SERV).
     induction k; first by apply positive_service_during in SERV.
     feed IHk; first by apply ltn_trans with k.+1.
     move: IHk => [t [/andP [NEQ1 NEQ2] [SCHEDt SERVk]]].
     have SERVk1: service_during sched j t1 t.+1 = k.+1.
     { rewrite -(service_during_cat _ _ _ t); last by apply/andP; split.
       rewrite  SERVk -[X in _ = X]addn1; apply/eqP; rewrite eqn_add2l.
-        by rewrite /service_during big_nat1 /service_at eqb1 -scheduled_at_def/=.  
-    } 
+      rewrite /service_during big_nat1 service_at_def /=.
+      by rewrite eqb1 -scheduled_at_def /=.
+    }
     move: SERV; rewrite -(service_during_cat _ _ _ t.+1); last first.
     { by apply/andP; split; first apply leq_trans with t. }
     rewrite SERVk1 -addn1 leq_add2l; move => SERV.
     destruct (scheduled_at sched j t.+1) eqn:SCHED.
     - exists t.+1; repeat split; try done. apply/andP; split.
-      + apply leq_trans with t; by done. 
+      + apply leq_trans with t; by done.
       + rewrite ltnNge; apply/negP; intros CONTR.
           by move: SERV; rewrite /service_during big_geq.
     -  apply negbT in SCHED.
        move: SERV; rewrite /service /service_during; move => /sum_seq_gt0P [x [INx SCHEDx]].
-       rewrite lt0b in SCHEDx.
+       rewrite service_at_def lt0b in SCHEDx.
        rewrite mem_iota subnKC in INx; last by done.
        move: INx => /andP [INx1 INx2].
        move: (exists_first_intermediate_point _ _ _ INx1 SCHED) => A.
        feed A; first by rewrite scheduled_at_def/=.
        move: A => [y [/andP [T1 T4] [T2 T3]]].
-       exists y; repeat split; try done.
+       exists y; repeat split => //.
        + apply/andP; split.
-         apply leq_trans with t; first by done. 
+         apply leq_trans with t; first by done.
          apply ltnW, ltn_trans with t.+1; by done.
-           by apply leq_ltn_trans with x. 
+           by apply leq_ltn_trans with x.
        + rewrite (@big_cat_nat _ _ _ t.+1) //=; [ | by apply leq_trans with t | by apply ltn_trans with t.+1].
          unfold service_during in SERVk1; rewrite SERVk1; apply/eqP.
          rewrite -{2}[k.+1]addn0 eqn_add2l.
          rewrite big_nat_cond big1 //; move => z /andP [H5 _].
-           by apply/eqP; rewrite eqb0; specialize (T2 z); rewrite scheduled_at_def/= in T2; apply T2.
+         apply/eqP.
+         rewrite service_at_def eqb0.
+         by specialize (T2 z); rewrite scheduled_at_def/= in T2; apply T2.
   Qed.
 
 End IncrementalService.
 
 (** * Automation *)
-(** We add the above lemmas into a "Hint Database" basic_facts, so Coq 
+(** We add the above lemmas into a "Hint Database" basic_facts, so Coq
     will be able to apply them automatically. *)
 Global Hint Resolve ideal_proc_model_is_a_uniprocessor_model
      ideal_proc_model_ensures_ideal_progress
@@ -202,19 +255,19 @@ Global Hint Resolve ideal_proc_model_is_a_uniprocessor_model
 
 (** We also provide tactics for case analysis on ideal processor state. *)
 
-(** The first tactic generates two sub-goals: one with idle processor and 
+(** The first tactic generates two sub-goals: one with idle processor and
     the other with processor executing a job named [JobName]. *)
 Ltac ideal_proc_model_sched_case_analysis sched t JobName :=
   let Idle := fresh "Idle" in
   let Sched := fresh "Sched_" JobName in
   destruct (ideal_proc_model_sched_case_analysis sched t) as [Idle | [JobName Sched]].
 
-(** The second tactic is similar to the first, but it additionally generates 
+(** The second tactic is similar to the first, but it additionally generates
     two equalities: [sched t = None] and [sched t = Some j]. *)
 Ltac ideal_proc_model_sched_case_analysis_eq sched t JobName :=
   let Idle := fresh "Idle" in
   let IdleEq := fresh "Eq" Idle in
-  let Sched := fresh "Sched_" JobName in 
+  let Sched := fresh "Sched_" JobName in
   let SchedEq := fresh "Eq" Sched in
   destruct (ideal_proc_model_sched_case_analysis sched t) as [Idle | [JobName Sched]];
   [move: (Idle) => /eqP IdleEq; rewrite ?IdleEq
